examples/sess/impl.v
@@ -1,0 +1,29 @@
+From stdpp Require Import base gmap.
+From mathcomp Require Import ssreflect.
+From stdpp Require Import namespaces.
+From iris.algebra Require Import agree auth csum gset gmap excl frac.
+From iris.algebra Require Import max_prefix_list.
+From iris.heap_lang Require Import notation proofmode.
+From cryptis Require Import lib term cryptis primitives tactics.
+From cryptis Require Import role iso_dh gen_conn.
+
+Set Implicit Arguments.
+Unset Strict Implicit.
+Unset Printing Implicit Defensive.
+
+Definition connect : val := λ: "c" "skA" "pkB" "N",
+  GenConn.connect "c" "skA" "pkB" "N".
+
+Definition listen : val := λ: "c", GenConn.listen "c".
+
+Definition confirm : val := λ: "c" "skB" "N" "req",
+  GenConn.confirm "c" "skB" "N" "req".
+
+Definition send : val := λ: "c" "m",
+  GenConn.send "c" "m".
+
+Definition recv : val := λ: "c",
+  (* FIXME: This step is used to add an extra later credit during the proof, but
+     it should be possible to remove it.  *)
+  let: <> := #() in
+  GenConn.recv "c".
