examples/sess/proofs.v
@@ -1,0 +1,134 @@
+From stdpp Require Import base gmap.
+From mathcomp Require Import ssreflect.
+From stdpp Require Import namespaces.
+From iris.algebra Require Import agree auth csum gset gmap excl frac.
+From iris.algebra Require Import max_prefix_list.
+From iris.heap_lang Require Import notation proofmode.
+From cryptis Require Import lib term gmeta cryptis primitives tactics role.
+From cryptis.examples Require Import iso_dh gen_conn.
+From cryptis.examples.sess Require impl.
+From cryptis.examples.sess.proofs Require Import base.
+From actris.channel Require Import proto_model proto.
+
+Set Implicit Arguments.
+Unset Strict Implicit.
+Unset Printing Implicit Defensive.
+
+Section Proofs.
+
+Context `{!cryptisGS Σ, !heapGS Σ, !iso_dhGS Σ, !GenConn.connGS Σ, !sessG Σ}.
+Notation iProp := (iProp Σ).
+
+Implicit Types (cs : GenConn.state).
+Implicit Types (skI skR : sign_key) (kS t : term).
+Implicit Types n : nat.
+Implicit Types γ : gname.
+Implicit Types v : val.
+
+Notation sessN := (iso_dhN.@"res".@"sess").
+
+Lemma wp_connect P N p c skI skR :
+  channel c -∗
+  cryptis_ctx -∗
+  ctx N p -∗
+  minted skI -∗
+  minted skR -∗
+  {{{ GenConn.failure skI skR ∨ P }}}
+    impl.connect c skI (Spec.pkey skR) (Tag N)
+  {{{ cs, RET (repr cs);
+      connected skI skR Init cs p ∗
+      release_token (si_init_share cs) ∗
+      (public (si_key cs) ∨ P) }}}.
+Proof.
+iIntros "#? #? #? #? #? % !> P post".
+wp_lam; wp_pures. iApply wp_fupd.
+wp_apply (GenConn.wp_connect with "[] [P]"); eauto 10.
+iIntros "%cs (connected & P & own & rel & token)".
+iApply ("post" $! cs).
+by iFrame.
+Qed.
+
+Lemma wp_listen c N p :
+  channel c -∗
+  cryptis_ctx -∗
+  ctx N p -∗
+  {{{ True }}}
+    impl.listen c
+  {{{ ga skI, RET (ga, Spec.pkey skI)%V;
+      public ga ∗ minted skI }}}.
+Proof.
+iIntros "#? #? #? % !> _ post".
+wp_lam. by iApply GenConn.wp_listen.
+Qed.
+
+Lemma wp_confirm P N p c skI skR ga :
+  channel c -∗
+  cryptis_ctx -∗
+  ctx N p -∗
+  {{{ public ga ∗ minted skI ∗ minted skR ∗
+      (GenConn.failure skI skR ∨ P) }}}
+    impl.confirm c skR (Tag N) (ga, Spec.pkey skI)%V
+  {{{ cs, RET (repr cs);
+      connected skI skR Resp cs (iProto_dual p) ∗
+      (public (si_key cs) ∨ P) }}}.
+Proof.
+iIntros "#? #ctx1 #? !> %Φ (#p_ga & #m_skI & #m_skR & P) post".
+wp_lam; wp_pures. iApply wp_fupd.
+wp_apply (GenConn.wp_confirm P with "[] [$P]").
+- eauto.
+- eauto.
+- do 3!iSplit => //.
+  iIntros "!> %b tok".
+  iMod (iProto_init p) as (γl γr) "(ctx & ownI & ownR)".
+  iMod (term_meta_set (sessN.@"names") (γl, γr) with "tok") as "#meta".
+  { solve_ndisj. }
+  iModIntro. iSplitL "ownI".
+  { iExists (γl, γr). iFrame. by eauto. }
+  iSplitL "ownR".
+  { iExists (γl, γr). iFrame. by eauto. }
+  iExists (γl, γr). iFrame. by eauto.
+iIntros "%cs (conn & dis & proto & rel & token)".
+iApply "post". by iFrame.
+Qed.
+
+Lemma wp_send skI skR rl cs (t : term) N p0 p :
+  ctx N p0 ∗ public t -∗
+  {{{ connected skI skR rl cs (<!> MSG t; p) }}}
+    impl.send (repr cs) t
+  {{{ RET #(); connected skI skR rl cs p }}}.
+Proof.
+iIntros "#(ctx & p_t) !>"; iIntros (Φ) "[c own] post". wp_lam; wp_pures.
+wp_apply (GenConn.wp_send_fupdN (λ skI skR si, sess_own skI skR si rl p)
+           with "[//] [//] [$c own]").
+{ iDestruct "own" as "[#fail|own]"; eauto.
+  iRight. iIntros (ts_send ts_recv) "inv".
+  iMod (sess_send with "own inv") as "upd". by iIntros "!>". }
+iIntros "[??]"; iApply "post". by iFrame.
+Qed.
+
+Lemma wp_recv {TT : tele} skI skR rl cs N p0
+  (t : TT → term) (P : TT → iProp) (p : TT → iProto Σ term) :
+  ctx N p0 -∗
+  {{{ connected skI skR rl cs (<?.. x> MSG t x {{ P x }}; p x) }}}
+    impl.recv (repr cs)
+  {{{ t', RET (repr t'); public t' ∗ (public (si_key cs) ∨
+      ∃.. x, ⌜t' = t x⌝ ∗ connected skI skR rl cs (p x) ∗ P x) }}}.
+Proof.
+iIntros "#ctx !>"; iIntros (Φ) "[c own] post".
+rewrite /impl.recv. wp_pure _ credit:"c1". wp_pure _ credit:"c2".
+wp_pures.
+wp_apply (GenConn.wp_recv (λ skI skR si (t' : term),
+                           ∃.. x, ⌜t' = t x⌝ ∗
+                                  sess_own skI skR si rl (p x) ∗ P x)%I
+           with "[//] [$c c1 c2 own]").
+{ iDestruct "own" as "[#fail|own]"; eauto.
+  iRight. iIntros (t' ts_send ts_recv) "inv".
+  iMod (sess_recv with "[$c1 $c2] own inv") as "[??]".
+  iModIntro. by iFrame. }
+iIntros "%t' (conn & #p_t' & inv)". iApply "post".
+iSplit => //. iDestruct "inv" as "[#fail|inv]"; eauto. iRight.
+iDestruct "inv" as (x) "(-> & own & Px)". iExists x. iFrame.
+by eauto.
+Qed.
+
+End Proofs.
