examples/sess/proofs/base.v
@@ -1,0 +1,156 @@
+From stdpp Require Import base gmap.
+From mathcomp Require Import ssreflect.
+From stdpp Require Import namespaces coGset.
+From iris.algebra Require Import agree auth csum gset gmap excl frac.
+From iris.algebra Require Import max_prefix_list.
+From iris.algebra.lib Require Import dfrac_agree.
+From iris.base_logic.lib Require Import invariants.
+From iris.heap_lang Require Import notation proofmode.
+From iris.heap_lang.lib Require Import ticket_lock.
+From cryptis Require Import lib term gmeta nown saved_prop.
+From cryptis Require Import cryptis primitives tactics role.
+From cryptis.examples Require Import iso_dh gen_conn.
+From actris.channel Require Import proto_model proto.
+
+Set Implicit Arguments.
+Unset Strict Implicit.
+Unset Printing Implicit Defensive.
+
+Notation sessN := (iso_dhN.@"res".@"sess").
+
+Definition savedProtoR Σ V :=
+  agreeR (laterO (iProto Σ V)).
+
+Definition savedProtoΣ V := #[
+  GFunctor (agreeRF (laterOF (protoOF (leibnizO V) idOF idOF)))
+].
+
+Class savedProtoG Σ V := savedProtoG_inG :: inG Σ (savedProtoR Σ V).
+
+Class sessG Σ := SessG {
+  #[local] sessG_protoG :: protoG Σ term;
+  #[local] sessG_agreeG :: savedProtoG Σ term;
+}.
+
+Definition sessΣ := #[
+  protoΣ term;
+  savedProtoΣ term
+].
+
+Global Instance subG_sess Σ : subG sessΣ Σ → sessG Σ.
+Proof. solve_inG. Qed.
+
+Section Verif.
+
+Context `{!cryptisGS Σ, !heapGS Σ, !iso_dhGS Σ, !GenConn.connGS Σ, !sessG Σ}.
+Notation iProp := (iProp Σ).
+
+Implicit Types (skI skR : sign_key) (kS t : term) (ts : list term).
+Implicit Types n : nat.
+Implicit Types b : bool.
+Implicit Types v : val.
+Implicit Types (ok : Prop) (failed : bool).
+Implicit Types si : sess_info.
+Implicit Types (N : namespace) (E : coPset) (p : iProto Σ term).
+Implicit Types γ : gname.
+
+Definition session_names si (γs : gname * gname) : iProp :=
+  term_meta (si_resp_share si) (sessN.@"names") γs.
+
+Definition session_name_for rl : gname * gname → gname :=
+  if rl is Init then fst else snd.
+
+Lemma session_names_agree si γs1 γs2 :
+  session_names si γs1 -∗
+  session_names si γs2 -∗
+  ⌜γs1 = γs2⌝.
+Proof. iApply term_meta_agree. Qed.
+
+Definition sess_own skI skR si (rl : role) p : iProp :=
+  ∃ γs,
+    session_names si γs ∗
+    iProto_own (session_name_for rl γs) p.
+
+Definition sess_ctx skI skR si tsI tsR : iProp :=
+  ∃ γs,
+    session_names si γs ∗
+    iProto_ctx γs.1 γs.2 tsI tsR.
+
+Definition sess_params p := {|
+  GenConn.init_pred := λ skI skR si rl,
+    sess_own skI skR si rl (if rl is Init then p else iProto_dual p);
+  GenConn.chan_inv := sess_ctx;
+|}%I.
+
+Lemma sess_send p0 skI skR si rl t p ts_send ts_recv :
+  sess_own skI skR si rl (<!> MSG t; p) -∗
+  ▷ GenConn.chan_inv_for (sess_params p0) skI skR si rl ts_send ts_recv
+  ={⊤ ∖ ↑GenConn.connN, ∅}=∗ |={∅}▷=>^(S (length ts_recv)) |={∅, ⊤ ∖ ↑GenConn.connN}=>
+    GenConn.chan_inv_for (sess_params p0) skI skR si rl (ts_send ++ [t]) ts_recv ∗
+    sess_own skI skR si rl p.
+Proof.
+iIntros "(%γs & #Hγs & own) (%γs' & >#Hγs' & ctx)".
+iPoseProof (session_names_agree with "Hγs Hγs'") as "<-".
+iClear "Hγs'". case: rl => /=.
+- iApply fupd_mask_intro; first set_solver.
+  iIntros "close !> !>".
+  iMod (iProto_send with "ctx own []") as "[ctx own]".
+  { rewrite iMsg_base_eq /=; eauto. }
+  iApply step_fupdN_intro => //.
+  iIntros "!> !>". iMod "close" as "_".
+  iModIntro. by iFrame; eauto.
+- rewrite iProto_ctx_sym.
+  iApply fupd_mask_intro; first set_solver.
+  iIntros "close !> !>".
+  iMod (iProto_send with "ctx own []") as "[ctx own]".
+  { rewrite iMsg_base_eq /=; eauto. }
+  iApply step_fupdN_intro => //.
+  iIntros "!> !>". iMod "close" as "_".
+  iModIntro. rewrite iProto_ctx_sym. by iFrame; eauto.
+Qed.
+
+Lemma sess_recv {TT : tele} p0 skI skR si rl t'
+  (t : TT → term) (P : TT → iProp) (p : TT → iProto Σ term) ts_send ts_recv :
+  £ 1 ∗ £ 1 -∗
+  sess_own skI skR si rl (<?.. x> MSG t x {{ P x }}; p x) -∗
+  ▷ GenConn.chan_inv_for (sess_params p0) skI skR si rl ts_send (t' :: ts_recv)
+  ={⊤ ∖ ↑GenConn.connN}=∗
+    ▷ (GenConn.chan_inv_for (sess_params p0) skI skR si rl ts_send ts_recv ∗
+       ∃.. x, ⌜t' = t x⌝ ∗ sess_own skI skR si rl (p x) ∗ P x).
+Proof.
+iIntros "[c1 c2] (%γs & #Hγs & own) (%γs' & >#Hγs' & ctx)".
+iPoseProof (session_names_agree with "Hγs Hγs'") as "<-".
+iClear "Hγs'". case: rl => /=.
+- iMod (lc_fupd_elim_later with "c1 ctx") as "ctx".
+  iMod (iProto_recv with "ctx own") as "(%p' & ctx & own & Ht')".
+  rewrite iMsg_base_eq /=.
+  iMod (lc_fupd_elim_later with "c2 Ht'") as "Ht'".
+  iDestruct (iMsg_texist_exist with "Ht'") as (x <-) "[Hp' HP]".
+  iIntros "!> !>".
+  iFrame. iSplit => //. iExists x. iFrame. iSplit => //.
+  iExists _. iSplit; eauto. by iRewrite "Hp'".
+- rewrite iProto_ctx_sym.
+- iMod (lc_fupd_elim_later with "c1 ctx") as "ctx".
+  iMod (iProto_recv with "ctx own") as "(%p' & ctx & own & Ht')".
+  rewrite iMsg_base_eq /=.
+  iMod (lc_fupd_elim_later with "c2 Ht'") as "Ht'".
+  iDestruct (iMsg_texist_exist with "Ht'") as (x <-) "[Hp' HP]".
+  iIntros "!> !>". rewrite iProto_ctx_sym.
+  iFrame. iSplit => //. iExists x. iFrame. iSplit => //.
+  iExists _. iSplit; eauto. by iRewrite "Hp'".
+Qed.
+
+Definition connected skI skR rl cs p : iProp :=
+  GenConn.connected (sess_params p) skI skR rl cs ∗
+  (public (si_key cs) ∨ sess_own skI skR cs rl p).
+
+Definition ctx N p := GenConn.ctx N (sess_params p).
+
+Lemma ctx_alloc N p E :
+  ↑N ⊆ E →
+  GenConn.pre_ctx -∗
+  iso_dh_token E ==∗
+  ctx N p ∗ iso_dh_token (E ∖ ↑N).
+Proof. exact: GenConn.ctx_alloc. Qed.
+
+End Verif.
